regmachine.v
@@ -73,10 +73,11 @@ Definition reg := nat.
 
 (* Instruction Set *)
 Inductive instr :=
-| WriteReg : V -> reg -> instr
-| ReadLoc  : reg -> loc -> instr
-| WriteLoc : V -> loc -> instr
-| CJmp     : reg -> nat -> instr.
+| WriteReg of V   & reg 
+| ReadLoc  of reg & loc
+| WriteLoc of V   & loc 
+| CJmp     of reg & nat 
+| Stop.
 
 Definition seqprog := seq instr.
 
@@ -108,7 +109,7 @@ Record config := Config {
   trhdmap  :> {fsfun E -> (thrd_state * nat)%type with (init_state, 0)}
 }.
 
-Notation inth := (nth (CJmp 0 0)).
+Notation inth := (nth Stop).
 
 Definition thrd_sem (pgm : seqprog) (st : thrd_state) :
   (option (@label unit V) * (V -> thrd_state))%type :=
@@ -129,6 +130,7 @@ Definition thrd_sem (pgm : seqprog) (st : thrd_state) :
     | CJmp     r n => (None,
                       fun _ => {| ip     := if rmap r != inh then n.+1 else ip.+1;
                                   regmap := rmap |} )
+    | Stop         => (None, fun=> st)
     end.
 
 Definition ltr_thrd_sem (l : option (@label V V)) pgm st1 st2 : bool :=
@@ -175,11 +177,11 @@ Definition es_seq x {pr} : (seq (exec_event_struct * E)) :=
       let: w_in     := valP w in
       let: read_lab := Read x (wval (lab es wr)) in
       (
-        add_event
+        add_new_event
           {| add_lb            := read_lab;
-            add_pred_in_dom   := pr_mem;
-            add_write_in_dom  := ws_mem   w_in;
-            add_write_consist := ws_wpred w_in; |},
+             add_pred_in_dom   := pr_mem;
+             add_write_in_dom  := ws_mem   w_in;
+             add_write_consist := ws_wpred w_in; |},
         wr
       ) | w <- (seq_in (writes_seq x))]
   else [::].
@@ -195,6 +197,7 @@ Lemma mem_ces_seq_aux x pr ces:
 Proof.
   case: ces => ces w; rewrite mem_filter /= /es_seq => /andP[?].
   case: eqP=> // ? /mapP[?? [/[dup] C -> ws]].
+  move: C. rewrite /add_new_event; case: ifP=> _ C; first by case: es.
   apply/consist_add_event=> /=; first by case: es.
   by rewrite -C -ws.
 Qed.
@@ -207,7 +210,7 @@ Definition ces_seq x pr :=
     (Consist (mem_ces_seq_aux ces_mem), wval (lab es w)) | 
     ces_w_mem <- seq_in (@ces_seq_aux x pr)].
 
-Arguments consist_Nread {_ _ _}.
+Arguments consist_new_Nread {_ _ _}.
 
 Definition add_hole
   (l : @label unit V) pr :
@@ -215,9 +218,9 @@ Definition add_hole
   if pr \in fresh_id :: dom es =P true is ReflectT pr_mem then
     match l with
     | Write x v => 
-      [:: (Consist (consist_Nread es pr (Write x v) erefl pr_mem), v)]  
+      [:: (Consist (consist_new_Nread es pr (Write x v) erefl pr_mem), v)]  
     | ThreadStart =>
-      [:: (Consist (consist_Nread es pr ThreadStart erefl pr_mem), inh)]
+      [:: (Consist (consist_new_Nread es pr ThreadStart erefl pr_mem), inh)]
     | Read x __ => ces_seq x pr
     | _         => [::]
     end
